coq/TypedParsing.v
@@ -1,0 +1,689 @@
+(*! Frontend | Parser for the typed Kôika EDSL !*)
+Require Import
+        Koika.Common
+        Koika.TypedSyntax
+        Koika.IdentParsing.
+
+Export Koika.Types.SigNotations.
+Export Koika.Primitives.PrimTyped.
+Export Coq.Strings.String.
+Export Coq.Lists.List.ListNotations.
+
+Declare Custom Entry tkoika.
+Declare Custom Entry tkoika_args.
+Declare Custom Entry tkoika_var.
+Declare Custom Entry tkoika_types.
+Declare Custom Entry tkoika_branches.
+Declare Custom Entry tkoika_consts.
+
+Notation "'<{' e '}>'" :=
+  (e)
+    (e custom tkoika at level 200,
+     format "'<{' '[v' '/' e '/' ']' '}>'").
+
+(* Koika_consts *)
+Notation "'1'" :=
+  (Ob~1)
+    (in custom tkoika_consts at level 0).
+Notation "'0'" :=
+  (Ob~0)
+    (in custom tkoika_consts at level 0).
+
+Notation "bs '~' '0'" :=
+  (Bits.cons false bs)
+    (in custom tkoika_consts at level 7,
+        left associativity,
+        format "bs '~' '0'").
+Notation "bs '~' '1'" :=
+  (Bits.cons true bs)
+    (in custom tkoika_consts at level 7,
+        left associativity,
+        format "bs '~' '1'").
+Notation "'Ob' '~' number" :=
+  (Const (tau := bits_t _) number)
+    (in custom tkoika at level 7,
+        number custom tkoika_consts at level 99,
+        format "'Ob' '~' number").
+
+Notation "'|' a '`d' b '|'" :=
+  (Const (tau := bits_t a) (Bits.of_N a b%N))
+    (in custom tkoika,
+        a constr at level 0,
+        b constr at level 0,
+        format "'|' a '`d' b '|'").
+
+(* Koika_args *)
+Declare Custom Entry tkoika_middle_args.
+
+Notation "x" :=
+  (CtxCons _ x CtxEmpty)
+    (in custom tkoika_middle_args at level 0,
+        x custom tkoika at level 99).
+
+Notation "x ',' y" :=
+  (CtxCons _ x y)
+    (in custom tkoika_middle_args at level 1,
+        x custom tkoika_middle_args,
+        y custom tkoika_middle_args,
+        right associativity).
+
+Notation "'()'" :=
+  CtxEmpty (in custom tkoika_args).
+
+Notation "'(' x ')'" :=
+  x (in custom tkoika_args, x custom tkoika_middle_args).
+(* Koika_var *)
+
+(* Class NameRef := nr_name: string. *)
+(* Hint Extern 1 NameRef => serialize_ident_in_context : typeclass_instances. *)
+
+(* Notation ident_to_string' a := (match __Ltac2_Mark return NameRef with *)
+(*                                | a => _ *)
+(*                                end) (only parsing). *)
+
+Notation "a" :=
+  (ident_to_string a)
+    (in custom tkoika_var at level 0, a constr at level 0, format "'[' a ']'", only parsing).
+Notation "a" :=
+  (a)
+    (in custom tkoika_var at level 0, a constr at level 0, format "'[' a ']'", only printing).
+
+(* Koika_types *)
+Notation " '(' x ':' y ')'" :=
+  (cons (prod_of_argsig {| arg_name := x%string; arg_type := y |}) nil)
+    (in custom tkoika_types at level 60,
+        x custom tkoika_var at level 0,
+        y constr at level 12).
+Notation "a  b" :=
+  (app a b)
+    (in custom tkoika_types at level 95,
+        a custom tkoika_types,
+        b custom tkoika_types,
+        right associativity).
+
+(* Koika_branches *)
+Notation "x '=>' a " :=
+  (cons (x, a) nil)
+    (in custom tkoika_branches at level 60,
+        x custom tkoika at level 99,
+        a custom tkoika at level 89).
+Notation "arg1 '|' arg2" :=
+  (app arg1 arg2)
+    (in custom tkoika_branches at level 13,
+        arg1 custom tkoika_branches,
+        arg2 custom tkoika_branches,
+        format "'[v' arg1 ']' '/' '|'  '[v' arg2 ']'").
+
+(* Koika *)
+
+Notation "'fail'" :=
+  (Fail _)
+    (in custom tkoika, format "'fail'").
+Notation "'fail' '(' t ')'" :=
+  (Fail (bits_t t))
+    (in custom tkoika,
+        t constr at level 0,
+        format "'fail' '(' t ')'").
+Notation "'fail' '@(' t ')'" :=
+  (Fail t)
+    (in custom tkoika,
+        t constr at level 0,
+        format "'fail' '@(' t ')'").
+
+Require Import Magic.
+
+Notation "'pass'" :=
+  (Const (tau := bits_t 0) Ob)
+    (in custom tkoika).
+Notation "'magic'" :=
+  (Const __magic__)
+    (in custom tkoika).
+
+Notation "'let' a ':=' b 'in' c" :=
+  (Bind a b c)
+    (in custom tkoika at level 91,
+        a custom tkoika_var at level 1,
+        right associativity,
+        format "'[v' 'let'  a  ':='  b  'in' '/' c ']'").
+Notation "a ';' b" :=
+  (Seq a b)
+    (in custom tkoika at level 90,
+        format "'[v' a ';' '/' b ']'" ).
+Notation "'set' a ':=' b" :=
+  (Assign (k := a) _ b)
+    (in custom tkoika at level 89,
+        a custom tkoika_var at level 1,
+        format "'set'  a  ':='  b").
+Notation "'(' a ')'" :=
+  (a)
+    (in custom tkoika at level 1,
+        a custom tkoika,
+        format "'[v' '(' a ')' ']'").
+
+(* Notation "instance  '.(' method ')' args" := *)
+(*   (USugar (UCallModule instance _ method args)) *)
+(*     (in custom tkoika at level 1, *)
+(*         instance constr at level 0, *)
+(*         method constr, *)
+(*         args custom tkoika_args at level 99). *)
+(* Notation "'{' method '}' args" := *)
+(*   (USugar (UCallModule id _ method args)) *)
+(*     (in custom tkoika at level 1, *)
+(*         method constr at level 200, *)
+(*         args custom tkoika_args at level 99, *)
+(*         only parsing). *)
+(* Notation "method args" := *)
+(*   (USugar (UCallModule id _ method args)) *)
+(*     (in custom tkoika at level 1, *)
+(*         method constr at level 0, *)
+(*         args custom tkoika_args at level 99, *)
+(*         only parsing). *)
+
+Notation "a" :=
+  (Var (k := a) _)
+  (* (match a with *)
+  (*  | k => Var (k := k) *)
+  (*            ltac:( *)
+  (*          lazymatch goal with *)
+  (*          | |- VarRef ?sig ?k _ => exact (projT2 (must (assoc k sig))) *)
+  (*          end) *)
+  (* end) *)
+    (in custom tkoika at level 1, a custom tkoika_var at level 0, only parsing).
+Notation "a" :=
+  (Var (k := a) _)
+    (in custom tkoika at level 1, a custom tkoika_var at level 0, only printing).
+
+Notation "'read0' '(' reg ')' " :=
+  (Read P0 reg)
+    (in custom tkoika,
+        reg constr,
+        format "'read0' '(' reg ')'").
+Notation "'read1' '(' reg ')' " :=
+  (Read P1 reg)
+    (in custom tkoika,
+        reg constr,
+        format "'read1' '(' reg ')'").
+Notation "'write0' '(' reg ',' value ')'" :=
+  (Write P0 reg value)
+    (in custom tkoika,
+        reg constr at level 13,
+        format "'write0' '(' reg ',' value ')'").
+Notation "'write1' '(' reg ',' value ')'" :=
+  (Write P1 reg value)
+    (in custom tkoika,
+        reg constr at level 13,
+        format "'write1' '(' reg ',' value ')'").
+
+(* FIXME: need better way to infer the argument in Const *)
+
+Notation "'if' a 'then' t 'else' f" :=
+  (If a t f)
+    (in custom tkoika at level 86,
+        right associativity,
+        format "'[v' 'if'  a '/' 'then'  t '/' 'else'  f ']'").
+Notation "'guard' '(' a ')' " :=
+  (If (Unop (Bits1 (Not 1)) a) (Fail (bits_t 0)) (Const (tau := bits_t 0) Ob))
+    (in custom tkoika at level 86,
+        right associativity,
+        format "'guard' '(' a ')'").
+Notation "'when' a 'do' t " :=
+  (If a t (Const (tau := bits_t 0) Ob))
+    (in custom tkoika at level 91,
+        right associativity,
+        format "'[v' 'when'  a '/' 'do'  t '/' ']'").
+
+Notation "a '&&' b" :=
+  (Binop (Bits2 (And _)) a b)
+    (in custom tkoika at level 80,
+        right associativity,
+        format "a  '&&'  b").
+Notation "'!' a" :=
+  (Unop (Bits1 (Not _)) a)
+    (in custom tkoika at level 75,
+        format "'!' a").
+Notation "a '||' b" :=
+  (Binop (Bits2 (Or _)) a b)
+    (in custom tkoika at level 85,
+        format "a  '||'  b").
+Notation "'zeroExtend(' a ',' b ')'" :=
+  (Unop (Bits1 (ZExtL _ b)) a)
+    (in custom tkoika,
+        b constr at level 0,
+        format "'zeroExtend(' a ',' b ')'").
+Notation "'sext(' a ',' b ')'" :=
+  (Unop (Bits1 (SExt _ b)) a)
+    (in custom tkoika,
+        b constr at level 0,
+        format "'sext(' a ',' b ')'").
+Notation "'ignore(' a ')'" :=
+  (Unop (Conv _ Ignore) a)
+    (in custom tkoika,
+        a custom tkoika).
+Notation "'pack(' a ')'" :=
+  (Unop (Conv _ Pack) a)
+    (in custom tkoika,
+        a custom tkoika).
+Notation "'unpack(' t ',' v ')'" :=
+  (Unop (Conv t Unpack) v)
+    (in custom tkoika,
+        t constr at level 11,
+        v custom tkoika).
+Notation "a  '^'  b" :=
+  (Binop (Bits2 (Xor _)) a b)
+    (in custom tkoika at level 85).
+Notation "a  '+'  b" :=
+  (Binop (Bits2 (Plus _)) a b)
+    (in custom tkoika at level 85).
+Notation "a  '-'  b" :=
+  (Binop (Bits2 (Minus _)) a b)
+    (in custom tkoika at level 85).
+Notation "a  '*'  b" :=
+  (Binop (Bits2 (Mul _ _)) a b)
+    (in custom tkoika at level 84).
+Notation "a  '!='  b" :=
+  (Binop (Eq _ true) a b)
+    (in custom tkoika at level 79).
+Notation "a  '=='  b" :=
+  (Binop (Eq _ false) a b)
+    (in custom tkoika at level 79).
+Notation "a  '>>'  b" :=
+  (Binop (Bits2 (Lsr _ _)) a b)
+    (in custom tkoika at level 79).
+Notation "a  '>>>'  b" :=
+  (Binop (Bits2 (Asr _ _)) a b)
+    (in custom tkoika at level 79).
+Notation "a  '<<'  b" :=
+  (Binop (Bits2 (Lsl _ _)) a b)
+    (in custom tkoika at level 79).
+Notation "a  '<'  b" :=
+  (Binop (Bits2 (Compare false cLt _)) a b)
+    (in custom tkoika at level 79).
+Notation "a  '<s'  b" :=
+  (Binop (Bits2 (Compare true cLt _)) a b)
+    (in custom tkoika at level 79).
+Notation "a  '<='  b" :=
+  (Binop (Bits2 (Compare false cLe _)) a b)
+    (in custom tkoika at level 79).
+Notation "a  '<s='  b" :=
+  (Binop (Bits2 (Compare true cLe _)) a b)
+    (in custom tkoika at level 79).
+Notation "a  '>'  b" :=
+  (Binop (Bits2 (Compare false cGt _)) a b)
+    (in custom tkoika at level 79).
+Notation "a  '>s'  b" :=
+  (Binop (Bits2 (Compare true cGt _)) a b)
+    (in custom tkoika at level 79).
+Notation "a  '>='  b" :=
+  (Binop (Bits2 (Compare false cGe _)) a b)
+    (in custom tkoika at level 79).
+Notation "a  '>s='  b" :=
+  (Binop (Bits2 (Compare true cGe _)) a b)
+    (in custom tkoika at level 79).
+Notation "a '++' b" :=
+  (Binop (Bits2 (Concat _ _)) a b)
+    (in custom tkoika at level 80,
+        right associativity,
+        format "a  '++'  b").
+Notation "a '[' b ']'" :=
+  (Binop (Bits2 (Sel _)) a b)
+    (in custom tkoika at level 75,
+        format "'[' a [ b ] ']'").
+(* Notation "a '[' b ':' c ']'" := *)
+(*    (Binop (Bits2 (IndexedSlice _ c)) a b) *)
+(*    (in custom tkoika at level 75, *)
+(*        c constr at level 0, *)
+(*        format "'[' a [ b ':' c ] ']'"). *)
+Notation "a '[' b ':+' c ']'" :=
+  (Binop (Bits2 (IndexedSlice _ c)) a b)
+    (in custom tkoika at level 75,
+        c constr at level 0,
+        format "'[' a [ b ':+' c ] ']'").
+Notation "'`' a '`'" :=
+  (a)
+    (in custom tkoika at level 99,
+        a constr at level 99).
+
+(* FIXME Hint Mode for VarRef *)
+Notation "'fun' nm args ':' ret '=>' body" :=
+  (@Build_InternalFunction'
+     string (action _ _ string _ _ (List.rev args) ret)
+     nm%string body)
+    (in custom tkoika at level 99,
+        nm custom tkoika_var at level 0,
+        args custom tkoika_types,
+        ret constr at level 0,
+        body custom tkoika at level 99,
+        format "'[v' 'fun'  nm  args  ':'  ret  '=>' '/' body ']'").
+
+Notation "'fun' nm '()' ':' ret '=>' body" :=
+  (@Build_InternalFunction'
+     string (action _ _ string _ _ (List.rev nil) ret)
+     nm%string body)
+    (in custom tkoika at level 99,
+        nm custom tkoika_var at level 0,
+        ret constr at level 0,
+        body custom tkoika at level 99,
+        format "'[v' 'fun'  nm  '()'   ':'  ret  '=>' '/' body ']'").
+
+(* Deprecated *)
+(* Notation "'call' instance method args" := *)
+(*   (USugar (UCallModule instance _ method args)) *)
+(*     (in custom tkoika at level 99, *)
+(*         instance constr at level 0, *)
+(*         method constr at level 0, *)
+(*         args custom tkoika_args). *)
+
+Notation "'funcall' method args" :=
+  (InternalCall method args)
+    (in custom tkoika at level 98,
+        method constr at level 0,
+        args custom tkoika_args).
+
+Notation "'extcall' method '(' arg ')'" :=
+  (ExternalCall method arg)
+    (in custom tkoika at level 98,
+        method constr at level 0,
+        arg custom tkoika).
+
+(* Notation "'call0' instance method " := *)
+(*   (USugar (UCallModule instance _ method nil)) *)
+(*     (in custom tkoika at level 98, *)
+(*         instance constr at level 0, *)
+(*         method constr). *)
+
+Notation "'funcall0' method " :=
+  (InternalCall _ method nil)
+    (in custom tkoika at level 98,
+        method constr at level 0).
+
+(* Definition str tau := *)
+(*   (must (match tau )) *)
+
+Section TypedMacros.
+  Context {pos_t var_t fn_name_t rule_name_t reg_t ext_fn_t: Type}.
+  Context {R: reg_t -> type}
+          {Sigma: ext_fn_t -> ExternalSignature}.
+  Context {REnv : Env reg_t}.
+
+  Notation action := (action pos_t var_t fn_name_t R Sigma).
+
+  Definition struct_sig_of_action {sig tau} (a: action sig tau)
+    : option struct_sig :=
+    match tau with
+    | struct_t sig => Some sig
+    | _ => None
+    end.
+
+  Definition init sig (tau: type) : action sig tau :=
+    let zeroes := Const (tau := bits_t _) (Bits.zeroes (type_sz tau)) in
+    Unop (Conv tau Unpack) zeroes.
+
+  Fixpoint struct_init
+           {sig}
+           (ssig: struct_sig)
+           (initializers: context (fun k_tau => action sig (snd k_tau))
+                            ssig.(struct_fields))
+    : action sig (struct_t ssig) :=
+    let empty := init sig (struct_t ssig) in
+    let mk_subst f := Binop (Struct2 SubstField ssig f) in
+    cfoldli (V := fun k_tau => action sig (snd k_tau))
+            (fun k_tau m a (acc: action sig (struct_t ssig)) =>
+               (mk_subst (existT _ k_tau m)) acc a)
+            initializers empty.
+
+  Fixpoint switch {vk vtau} {sig tau} (m: member (vk, vtau) sig)
+           (default: action sig tau)
+           (branches: list (action sig vtau * action sig tau)) : action sig tau :=
+    match branches with
+    | nil => default
+    | (label, action) :: branches =>
+      If (Binop (Eq _ false) (Var m) label)
+         action (switch m default branches)
+    end.
+End TypedMacros.
+
+Notation must_field sig f :=
+  (must (PrimTypeInference.find_field_opt sig f)).
+
+Notation must_field_of_action a f :=
+  (must_field (must (struct_sig_of_action a)) f).
+
+(* Class StructField (sig: struct_sig) (f: string) := *)
+(*   sf_idx : struct_index sig. *)
+
+(* Hint Extern 1 (StructField ?sig ?f) => exact (must_field sig f) : typeclass_instances. *)
+(* Hint Mode StructField + + : typeclass_instances. *)
+
+(* Notation "'get' '(' v ',' f ')'" := *)
+(*   (Unop (Struct1 GetField _ (_: StructField _ f)) v) *)
+(*     (in custom tkoika, *)
+(*         v custom tkoika at level 13, *)
+(*         f custom tkoika_var at level 0, *)
+(*         format "'get' '(' v ','  f ')'"). *)
+
+Notation "'getbits' '(' sig ',' v ',' f ')'" :=
+  (Unop (Bits1 (GetFieldBits sig (must_field sig f))) v)
+    (in custom tkoika,
+        sig constr at level 11,
+        v custom tkoika at level 13,
+        f custom tkoika_var at level 0,
+        format "'getbits' '(' sig ','  v ','  f ')'").
+
+(* Notation "'subst' '(' v ',' f ',' a ')'" := *)
+(*   (Binop (Struct2 SubstField _ (_: StructField _ f)) v a) *)
+(*     (in custom tkoika, *)
+(*         v custom tkoika at level 13, *)
+(*         a custom tkoika at level 13, *)
+(*         f custom tkoika_var at level 0, *)
+(*         format "'subst' '(' v ','  f ',' a ')'"). *)
+
+Notation "'substbits' '(' sig ',' v ',' f ',' a ')'" :=
+  (Binop (Bits2 (SubstFieldBits sig (must_field sig f))) v a)
+    (in custom tkoika,
+        sig constr at level 11,
+        v custom tkoika at level 13,
+        a custom tkoika at level 13,
+        f custom tkoika_var at level 0,
+        format "'substbits' '(' sig ','  v ','  f ',' a ')'").
+
+Declare Custom Entry tkoika_structs_init.
+
+Notation "f ':=' expr ';'  rest" :=
+  (CtxCons (f, _) expr rest)
+    (in custom tkoika_structs_init at level 20,
+        f custom tkoika_var at level 0,
+        expr custom tkoika at level 88,
+        rest custom tkoika_structs_init).
+
+Notation "f ':=' expr" :=
+  (CtxCons (f, _) expr CtxEmpty)
+    (in custom tkoika_structs_init at level 20,
+        f custom tkoika_var at level 0,
+        expr custom tkoika at level 88).
+
+Notation "'struct' sig '{' fields '}'" :=
+  (struct_init sig fields)
+    (in custom tkoika,
+        sig constr at level 0,
+        fields custom tkoika_structs_init at level 92).
+
+Notation "'enum' sig '{' name '}'" :=
+  (Const (tau := enum_t sig)
+         (vect_nth (sig.(enum_bitpatterns))
+                   (must (vect_index name sig.(enum_members)))))
+    (in custom tkoika at level 1,
+        sig constr at level 1,
+        name custom tkoika_var at level 1).
+
+Notation "'match' term 'with' '|' branches 'return' 'default' ':' default 'end'" :=
+  (Bind "__reserved__matchPattern" term
+        (switch (MemberHd ("__reserved__matchPattern", _) _)
+                default branches))
+    (in custom tkoika at level 30,
+        term custom tkoika,
+        branches custom tkoika_branches,
+        default custom tkoika,
+        format "'match'  term  'with' '/' '[v'  '|'  branches '/' 'return'  'default' ':' default ']' 'end'").
+
+Notation "'#' s" :=
+  (Const (tau := bits_t _) s)
+    (in custom tkoika at level 98,
+        s constr at level 0,
+        only parsing).
+
+Module Type Tests.
+  Parameter pos_t : Type.
+  Definition fn_name_t := string.
+
+  Inductive reg_t := data0 | data1.
+  Parameter ext_fn_t : Type.
+
+  Axiom data1_sz : nat.
+  Definition R (reg: reg_t): type :=
+    match reg with
+    | data0 => bits_t 32
+    | data1 => bits_t data1_sz
+    end.
+  Parameter Sigma: ext_fn_t -> ExternalSignature.
+
+  Notation action R Sigma := (action pos_t string fn_name_t R Sigma).
+
+  (* With that instead of the typeclass we'll need to propagate top-down everywhere. *)
+  (* Arguments Seq {pos_t var_t fn_name_t reg_t ext_fn_t}%type_scope {R Sigma}%function_scope {sig tau} &. *)
+
+  Definition test_2 : action R Sigma [("u", unit_t); ("v", unit_t)] _ :=
+    <{ u; v }>.
+  Definition test_3 : action R Sigma [("v", unit_t)] _ :=
+    <{ set v := magic }>.
+
+  Definition test_1 : action R Sigma [] (bits_t 3) :=
+    <{ let v := fail(2) in magic }>.
+  Definition test_1' : action R Sigma [] _ :=
+    <{ let v := fail(2) in v }>.
+  Definition test_2' : action R Sigma [] unit_t :=
+    <{ magic; magic }>.
+  Definition test_3' : action R Sigma [("v", unit_t)] unit_t :=
+    <{ set v := magic; magic }>.
+  Definition test_4 : action R Sigma [("v", unit_t)] _ :=
+    <{ magic; set v := magic }>.
+  Definition test_5 : action R Sigma [("v", unit_t)] unit_t :=
+    <{ let v := set v := magic in magic }>.
+  Definition test_6 : action R Sigma [("v", unit_t)] unit_t :=
+    <{ let v := set v := magic; pass in magic; magic }>.
+  Definition test_7 : action R Sigma [("v", unit_t)] unit_t :=
+    <{ (let v := (set v := magic); pass in magic; magic) }>.
+  Definition test_8 : action R Sigma [("v", unit_t)] unit_t :=
+    <{ (let v := set v := magic; pass in magic); magic }>.
+  Inductive test : Set := rData (n: nat).
+  Definition R_test (reg: test) := match reg with rData n => bits_t n end.
+  Definition test_9 : action R Sigma [] _ :=
+    <{ read0(data0) }>.
+  Definition test_10 : forall (idx: nat), action R_test Sigma [] (bits_t idx) :=
+    (fun idx => <{ read0(rData idx) }>).
+  Definition test_11 : action R Sigma [("v", unit_t)] unit_t :=
+    <{ (let v := read0(data0) in write0(data0, magic)); fail }>.
+  Definition test_12 : action R Sigma [] unit_t :=
+    <{ (let v := if fail then read0(data0) else fail in
+        write0(data0, magic)); fail }>.
+
+  (* We're using Program Definition to work around quirks of Coq's type system. The alternative would be to use bidirectionality hints, but it's not robust: it breaks e.g. when specifying the return type of a concatenation, because without the argument we can't check that the concatenation has the right size.  *)
+  (* Arguments Binop {pos_t}%type_scope {var_t fn_name_t reg_t ext_fn_t}%type_scope {R Sigma}%function_scope {sig} fn &. *)
+  (* Arguments Unop {pos_t var_t fn_name_t reg_t ext_fn_t}%type_scope {R Sigma}%function_scope {sig} fn &. *)
+  (* FIXME bidirectionality hints some examples fail. Using a typeclasses for ident parsing and Var resolution helps but doesn't solve the problem. *)
+
+  Definition test_14 : action R Sigma [("v", bits_t 1)] (bits_t 1) :=
+    <{ !v && v }>.
+  Definition test_14' : action R Sigma [("v", bits_t 1)] _ :=
+    <{ !(v && v) }>.
+  Goal test_14 <> test_14'. Proof. compute; congruence. Qed.
+
+  (* Arguments Write {pos_t var_t fn_name_t reg_t ext_fn_t}%type_scope {R Sigma}%function_scope {sig} port idx &. *)
+
+  Definition test_15 : action R Sigma [("v", _ (* inferred *))] _ :=
+    <{ write0(data0, v); unpack(_ (* inferred *), v) && read0(data0) }>.
+  Definition test_16 : action R Sigma [] _ :=
+    <{ !read0(data0) && !read0(data0) }>. (* works without knowing the size of data1 *)
+  Definition test_16' : action R Sigma [] _ :=
+    <{ read0(data0) && read0(data0) }>.
+  Definition test_17 : action R Sigma [] _ :=
+    <{ !read0(data1) && magic}>.
+
+  Program Definition test_18 : action R Sigma [("v", bits_t 32)] _ :=
+    <{ !read0(data0) && v }>.
+
+  Definition test_19 : action R Sigma [("v", bits_t 32); ("w", bits_t 5); ("x", bits_t 5)] _ :=
+    <{ v [#(Bits.of_nat _ 2)] && Ob~1 }>.
+  Program Definition test_20 : action R Sigma _ _ :=
+    <{ let v := |32`d0| in v[Ob~0~0~0~0~0] }> : action R Sigma [] _.
+
+  (* Using Program Definition makes finding type errors much nicer: *)
+  Program Definition broken : action R Sigma [("v", bits_t 32)] _ :=
+    <{ !read0(data0) && v && v[Ob~0] }>.
+  Next Obligation.
+    exact 32.
+  Defined.
+  Next Obligation. Admitted.
+  Next Obligation. Admitted.
+  Next Obligation. Admitted.
+  Next Obligation. Admitted.
+
+  Program Definition test_20' : action R Sigma [("v", bits_t 32)] _ :=
+    <{ (v[magic :+ 3] ++ v) && (v[magic :+ 35]) }>.
+  Program Definition test_20'' : action R Sigma [("v", bits_t 32); ("w", bits_t 16)] (bits_t 51) :=
+    <{ (v ++ w ++ v[magic :+ 3]) }>.
+
+  Notation InternalFunction sig tau := (InternalFunction pos_t string fn_name_t R Sigma sig tau).
+
+  Definition test_23 : InternalFunction _ _ :=
+    <{ fun test (arg1 : (bits_t 3)) (arg2 : bits_t 2) : bits_t 4 => magic }>.
+
+  Definition test_24 : forall sz: nat, InternalFunction _ _ :=
+    (fun sz => <{ fun test (arg1 : bits_t sz) (arg1 : bits_t sz) : bits_t sz  => magic}>).
+  Definition test_25 : forall sz: nat, InternalFunction _ _ :=
+    (fun sz => <{fun test (arg1 : bits_t sz ) : bits_t sz => let oo := pass >> pass in magic}>).
+  Definition test_26 : forall sz: nat, InternalFunction _ _ :=
+    (fun sz => <{ fun test () : bits_t sz  => magic }>).
+  Program Definition test_27 : action R Sigma [("w", bits_t 1)] _ :=
+    <{
+        (if !(read0(data0)[Ob~0~0~0~0~0]) then
+           write0(data0, |32`d0|);
+           let u := if (w == Ob~1) then w else w || w
+           in write0(data0, |32`d0|)
+         else
+           (ignore(read0(data0)); pass));
+        fail(4)
+    }>.
+  Definition test_28 : action R Sigma [("var", bits_t 5)] unit_t :=
+    <{
+      match var with
+      | magic => magic
+      return default: magic
+      end
+    }>.
+
+  Definition test_sig :=
+    {| struct_name := "test_sig";
+       struct_fields := [("foo", bits_t 2); ("bar", bits_t 32)] |}.
+
+  Program Definition test_30'' : action R Sigma [("v", bits_t 5)] _ :=
+    <{
+      struct test_sig { foo := v[#(Bits.of_nat 3 0) :+ 2];
+                        bar := |32`d98| }
+    }>.
+
+  Definition test_31'' : action R Sigma [("a", struct_t test_sig)] _ :=
+    <{
+        pack(a)
+    }>.
+
+  Program Definition test_31' : action R Sigma [("v", bits_t 5)] _ :=
+    <{
+      let a := struct test_sig { foo := v[#(Bits.of_nat 3 0) :+ 2];
+                                bar := |32`d98| } in
+      unpack(struct_t test_sig, pack(a))
+    }>.
+
+  (* Definition test_32 : action R Sigma [("v", struct_t test_sig)] _ := *)
+  (*   <{ subst(v, foo, <{ Ob~1~1 }>) *)
+  (*   }>. *)
+End Tests.
